\section{Appendix}
Here we add some theorems (with demonstrations or not) that may interest the reader.

% TODO: Add ref ML a probabilistic perspective page 119-120 and 
\begin{theorem}[Bayes rule for linear Gaussian systems]
\label{thm:bayes-rule-lin-gaussian-sys}

Given a linear Gaussian system:
\begin{equation}
\boxed{
\begin{aligned}
p(x) &= \mathcal{N} (x | \mu_x , \Sigma_x) \\
p(y | x) &= \mathcal{N} (y | Ax + b, \Sigma_y)
\end{aligned}
}
\end{equation}
the posterior $p(x|y)$ is given by the following:

\begin{equation}
p(x | y) = \mathcal{N} \left( x | \mu_{x | y}, \Sigma_{x | y} \right)
\end{equation}
where:

\begin{equation}
\Sigma_{x | y}^{-1} = \Sigma_x^{-1} + A^T \Sigma_y^{-1} A
\end{equation}

\begin{equation}
\mu_{x | y} = \Sigma_{x | y} \left[ A^T \Sigma_y^{-1} (y - b) + \Sigma_x^{-1} \mu_x \right]
\end{equation}

In addition, the normalization constant $p(y)$ is given by

\begin{equation}
p(y) = \mathcal{N} \left( y | A \mu_x + b, \Sigma_y + A \Sigma_x A^T \right)
\end{equation}
\end{theorem}

\begin{theorem}[Marginals and conditionals of an MVN]
\label{thm:marginals-and-conditionals-mvn}
Suppose \( x = (x_1, x_2) \) is jointly Gaussian with parameters
\begin{equation}
\mu = \begin{pmatrix}
\mu_1 \\
\mu_2
\end{pmatrix}, \quad
\Sigma = \begin{pmatrix}
\Sigma_{11} & \Sigma_{12} \\
\Sigma_{21} & \Sigma_{22}
\end{pmatrix}, \quad
\Lambda = \Sigma^{-1} = \begin{pmatrix}
\Lambda_{11} & \Lambda_{12} \\
\Lambda_{21} & \Lambda_{22}
\end{pmatrix}.
\end{equation}

Then the marginals are given by:
\begin{equation}
p(x_1) = \mathcal{N}(x_1 | \mu_1, \Sigma_{11}), \quad p(x_2) = \mathcal{N}(x_2 | \mu_2, \Sigma_{22}).
\end{equation}

The posterior conditional is given by:
\begin{equation}
p(x_1 | x_2) = \mathcal{N}(x_1 | \mu_{1|2}, \Sigma_{1|2}),
\end{equation}

where

\begin{align}
\mu_{1|2}
&= \mu_1 + \Sigma_{12} \Sigma_{22}^{-1} (x_2 - \mu_2)\\
&= \mu_1 - \Lambda_{11}^{-1} \Lambda_{12} (x_2 - \mu_2)\\
&=\Sigma_{1|2} \left( \Lambda_{11} \mu_1 - \Lambda_{12} (x_2 - \mu_2) \right)
\end{align}

\begin{equation}
\Sigma_{1|2} = \Sigma_{11} - \Sigma_{12} \Sigma_{22}^{-1} \Sigma_{21} = \Lambda_{11}^{-1}.
\end{equation}
\end{theorem}


% TODO: add properties of Gaussian distributions
